NLustre/Clocking/Properties.v
@@ -18,109 +18,114 @@ Module Type PROPERTIES
        (Import IsD : ISDEFINED Ids Op Syn Mem)
        (Import Par : PARENTS Ids Op Syn Clo).
 
-Lemma Is_free_in_clock_self_or_parent:
-  forall x ck,
-    Is_free_in_clock x ck
-    -> exists ck' b, ck = Con ck' x b \/ clock_parent (Con ck' x b) ck.
-Proof.
-  Hint Constructors clock_parent.
-  induction ck as [|? IH]; [now inversion 1|].
-  intro Hfree.
-  inversion Hfree as [|? ? ? ? Hfree']; clear Hfree; subst.
-  - exists ck, b; now auto.
-  - specialize (IH Hfree'); clear Hfree'.
-    destruct IH as [ck' [b' Hcp]].
-    exists ck', b'; right.
-    destruct Hcp as [Hcp|Hcp]; [rewrite Hcp| inversion Hcp]; now auto.
-Qed.
+  Lemma Is_free_in_clock_self_or_parent:
+    forall x ck,
+      Is_free_in_clock x ck
+      -> exists ck' b, ck = Con ck' x b \/ clock_parent (Con ck' x b) ck.
+  Proof.
+    Hint Constructors clock_parent.
+    induction ck as [|? IH]; [now inversion 1|].
+    intro Hfree.
+    inversion Hfree as [|? ? ? ? Hfree']; clear Hfree; subst.
+    - exists ck, b; now auto.
+    - specialize (IH Hfree'); clear Hfree'.
+      destruct IH as [ck' [b' Hcp]].
+      exists ck', b'; right.
+      destruct Hcp as [Hcp|Hcp]; [rewrite Hcp| inversion Hcp]; now auto.
+  Qed.
+  
+  Section Well_clocked.
 
-Section Well_clocked.
+    (** We work under a (valid) clocking environment *)
+    Variable vars : list (ident * clock).
+    Variable Hnd : NoDupMembers vars.
+    Variable Hwc : wc_env vars.
 
+    Theorem wc_equation_not_Is_free_in_clock:
+      forall eq x ck,
+        wc_equation vars eq
+        -> Is_defined_in_eq x eq
+        -> Has_clock_eq ck eq
+        -> ~Is_free_in_clock x ck.
+    Proof.
+      intros eq x' ck' Hwce Hdef Hhasck Hfree.
+      inversion Hwce as [x ck e Hcv Hexp Heq
+                        |xs ck f e Hvars Hexp Heq
+                        |x ck v' e Hcv Hexp].
+      - subst eq. inv Hdef. inv Hhasck.
+        pose proof (wc_env_var _ _ _ Hwc Hcv) as Hclock.
+        apply Is_free_in_clock_self_or_parent in Hfree.
+        destruct Hfree as (ck' & b & [Hck|Hck]).
+        + subst ck.
+          apply wc_clock_sub with (1:=Hwc) in Hclock.
+          pose proof (NoDupMembers_det _ _ _ _ Hnd Hcv Hclock) as Hloop.
+          apply clock_no_loops with (1:=Hloop).
+        + apply wc_clock_parent with (1:=Hwc) (2:=Hck) in Hclock.
+          apply wc_clock_sub with (1:=Hwc) in Hclock.
+          rewrite (NoDupMembers_det _ _ _ _ Hnd Hcv Hclock) in *.
+          apply clock_parent_parent' in Hck.
+          apply clock_parent_not_refl with (1:=Hck).
+      - subst eq. rename x' into x. inv Hdef. inv Hhasck.
+        match goal with H:List.In x xs |- _ => rename H into Hin end.
+        pose proof (In_Forall _ _ _ Hvars Hin) as Hcv.
+        pose proof (wc_env_var _ _ _ Hwc Hcv) as Hclock.
+        apply Is_free_in_clock_self_or_parent in Hfree.
+        destruct Hfree as (ck' & b & [Hck|Hck]).
+        + subst ck.
+          apply wc_clock_sub with (1:=Hwc) in Hclock.
+          pose proof (NoDupMembers_det _ _ _ _ Hnd Hcv Hclock) as Hloop.
+          apply clock_no_loops with (1:=Hloop).
+        + apply wc_clock_parent with (1:=Hwc) (2:=Hck) in Hclock.
+          apply wc_clock_sub with (1:=Hwc) in Hclock.
+          rewrite (NoDupMembers_det _ _ _ _ Hnd Hcv Hclock) in *.
+          apply clock_parent_parent' in Hck.
+          apply clock_parent_not_refl with (1:=Hck).
+      - subst eq. inv Hdef. inv Hhasck.
+        pose proof (wc_env_var _ _ _ Hwc Hcv) as Hclock.
+        apply Is_free_in_clock_self_or_parent in Hfree.
+        destruct Hfree as (ck' & b & [Hck|Hck]).
+        + subst ck.
+          apply wc_clock_sub with (1:=Hwc) in Hclock.
+          pose proof (NoDupMembers_det _ _ _ _ Hnd Hcv Hclock) as Hloop.
+          apply clock_no_loops with (1:=Hloop).
+        + apply wc_clock_parent with (1:=Hwc) (2:=Hck) in Hclock.
+          apply wc_clock_sub with (1:=Hwc) in Hclock.
+          rewrite (NoDupMembers_det _ _ _ _ Hnd Hcv Hclock) in *.
+          apply clock_parent_parent' in Hck.
+          apply clock_parent_not_refl with (1:=Hck).
+    Qed.
 
-(** We work under a (valid) clocking environment *)
-Variable C : clockenv.
-Variable Hwc: wc_env C.
+    Corollary wc_EqDef_not_Is_free_in_clock:
+      forall x ce ck,
+        wc_equation vars (EqDef x ck ce)
+        -> ~Is_free_in_clock x ck.
+    Proof.
+      intros x ce ck Hwce Hwt.
+      now eapply wc_equation_not_Is_free_in_clock;
+        eauto using Has_clock_eq.
+    Qed.
 
-Theorem wc_equation_not_Is_free_in_clock:
-  forall eq x ck,
-      wc_equation C eq
-    -> Is_defined_in_eq x eq
-    -> Has_clock_eq ck eq
-    -> ~Is_free_in_clock x ck.
-Proof.
-(* XXX: This proof is rather fragile *)
-  intros eq x ck Hwce Hdef Hhasck Hfree.
-  inversion Hwce as [x' ck' e Hcv Hexp Heq
-                    |x' ck' f e Hcv Hexp Heq
-                    |x' ck' v' e Hcv Hexp];
-    subst; inversion Hdef; inversion Hhasck; clear Hdef Hhasck; subst;
-      match goal with
-      | _: context[ EqApp _ _ _ _ ],
-        Hin: List.In ?x x' |- _ =>
-        (* Case: eq ~ EqApp *)
-        (assert (Hlen : 0 < length x')
-          by now destruct x'; inv Hin; apply Lt.lt_0_Sn);
-        pose proof (In_Forall _ _ _ Hcv Hin) as Hck_x;
-        simpl in *;
-        generalize (wc_env_vars _ _ _ Hlen Hwc Hcv)
-      | _ =>
-        (* Case: eq ~ EqDef or eq ~ EqFby *)
-        generalize (wc_env_var _ _ _ Hwc Hcv)
-      end;
-      intro Hclock;
-      apply Is_free_in_clock_self_or_parent in Hfree;
-      destruct Hfree as [ck [b [Hck|Hck]]];
-      try match goal with
-      | _ : _ = Con _ _ _ |- _ =>
-        rewrite Hck in *;
-          apply wc_clock_sub with (1:=Hwc) in Hclock;
-          match reverse goal with
-          | H: wc_var C _ _ |- _ => apply wc_var_det with (1:=H) in Hclock
-          end;
-          apply clock_no_loops with (1:=Hclock)
-      | _ : clock_parent _ _ |- _ =>
-        apply wc_clock_parent with (1:=Hwc) (2:=Hck) in Hclock;
-          apply wc_clock_sub with (1:=Hwc) in Hclock;
-          match reverse goal with
-          | H: wc_var C _ _ |- _ => apply wc_var_det with (1:=H) in Hclock
-          end;
-          apply clock_parent_parent' in Hck;
-          rewrite <-Hclock in Hck;
-          apply clock_parent_not_refl with (1 := Hck)
-      end.
-Qed.
+    Corollary wc_EqApp_not_Is_free_in_clock:
+      forall xs f le ck,
+        wc_equation vars (EqApp xs ck f le)
+        -> forall x, List.In x xs -> ~Is_free_in_clock x ck.
+    Proof.
+      intros x f le ck Hwce Hwt y Hinx.
+      now eapply wc_equation_not_Is_free_in_clock;
+        eauto using Is_defined_in_eq, Has_clock_eq.
+    Qed.
 
-Corollary wc_EqDef_not_Is_free_in_clock:
-  forall x ce ck,
-      wc_equation C (EqDef x ck ce)
-    -> ~Is_free_in_clock x ck.
-Proof.
-  intros x ce ck Hwce Hwt.
-  now eapply wc_equation_not_Is_free_in_clock;
-    eauto using Has_clock_eq.
-Qed.
+    Corollary wc_EqFby_not_Is_free_in_clock:
+      forall x v0 le ck,
+        wc_equation vars (EqFby x ck v0 le)
+        -> ~Is_free_in_clock x ck.
+    Proof.
+      intros x v0 le ck Hwce Hwt.
+      now eapply wc_equation_not_Is_free_in_clock;
+        eauto using Has_clock_eq.
+    Qed.
 
-Corollary wc_EqApp_not_Is_free_in_clock:
-  forall xs f le ck,
-      wc_equation C (EqApp xs ck f le)
-    -> forall x, List.In x xs -> ~Is_free_in_clock x ck.
-Proof.
-  intros x f le ck Hwce Hwt y Hinx.
-  now eapply wc_equation_not_Is_free_in_clock;
-    eauto using Is_defined_in_eq, Has_clock_eq.
-Qed.
-
-Corollary wc_EqFby_not_Is_free_in_clock:
-  forall x v0 le ck,
-      wc_equation C (EqFby x ck v0 le)
-    -> ~Is_free_in_clock x ck.
-Proof.
-  intros x v0 le ck Hwce Hwt.
-  now eapply wc_equation_not_Is_free_in_clock;
-    eauto using Has_clock_eq.
-Qed.
-
-End Well_clocked.
+  End Well_clocked.
 
 End PROPERTIES.
 
